\subsection*{55. Structure equations.}

These are immediately deduced from the general equations established in Chapter I. These are written
\nequ{3}{
(\omega^i)' &= [\omega^i \omega] + [\omega^k \omega_k^i] + \Omega^i,\\
\omega' &= \Omega,\\
(\omega_i^j)' &= [\omega_i^k \omega_k^j] + \Omega_i^j,
}
and between these $\Omega_i^j$ one has the relations
\uequ{
g_{ii} \Omega_j^i + g_{jj} \Omega_i^j =0,
}
or
\nequ{4}{
\Omega_{ij} + \Omega_{ji}=0.
}
The equations (3) may also be written
\nequ{3'}{
(\omega_i)' &= [\omega_i \omega] + [\omega_i^k \omega_k] + \Omega_i,\\
\omega' &= \Omega,\\
(\omega_{ij})' &= [\omega_i^k \omega_{kj}] + \Omega_i^j
 = [\omega_{ki} \omega_j^k] + \Omega_{ij}.
}

Finally, the equations \?{bring over}{traduisent} the conservation theorem are
\nequ{5}{
(\Omega^i)' + [\omega\Omega^i] - [\omega^i \Omega]
 + [\omega_k^i \Omega^k] - [\omega^k \Omega_k^i] = 0,\\
\Omega'=0,\\
(\Omega_i^j)' + [\omega_k^j \Omega_i^k] - [\omega_i^k \Omega_k^j] = 0,
}
or
\nequ{5'}{
(\Omega_i)' + [\omega\Omega_i] - [\omega_i \Omega]
 + [\omega_i^k \Omega^k] - [\omega_k \Omega_i^k] = 0,\\
\Omega'=0,\\
(\Omega_{ij})' + [\omega_j^k \Omega_{ik}] - [\omega_i^k \Omega_{kj}] = 0,
}